@prefix foaf: <http://xmlns.com/foaf/0.1/> .
@prefix rdf: <http://www.w3.org/1999/02/22-rdf-syntax-ns#> .
@prefix rdfs: <http://www.w3.org/2000/01/rdf-schema#> .
@prefix dct: <http://purl.org/dc/terms/> .
@prefix dc: <http://purl.org/dc/elements/1.1/> .
@prefix owl: <http://www.w3.org/2002/07/owl#> .
@prefix xsd: <http://www.w3.org/2001/XMLSchema#> .
@prefix cc: <http://creativecommons.org/ns#> .

@prefix odrs: <http://schema.theodi.org/odrs#> .

############################################################################
# General description of the ontology
############################################################################

<http://schema.theodi.org/odrs>
    a owl:Ontology;
    owl:versionInfo "0.1";
    dct:title "Open Data Rights Statement Vocabulary"@en;
    rdfs:label "Open Data Rights Statement Vocabulary";
    rdfs:comment """A vocabulary that supports the publication of Open Data by providing the means to capture machine-readable "rights statements", e.g. the licensing information, copyright notices and attribution requirements that are associated with the publication and re-use of a dataset.""";
    dct:created "2013-05-31"^^xsd:date;
    dct:modified "2013-07-15"^^xsd:date;
    foaf:maker <http://www.ldodds.com#me>.

<http://www.ldodds.com#me> a foaf:Person ;
    foaf:name "Leigh Dodds" .

############################################################################
# Classes
############################################################################

odrs:RightsStatement
    a owl:Class;    
    rdfs:isDefinedBy <http://schema.theodi.org/odrs>;
    rdfs:label "Rights Statement"@en;
    rdfs:comment """A description of how to re-use a dataset. A rights statement will include a reference to one or more licences, copyright notices, and attribution requirements. A Rights Statement provides additional context that qualifies the relationship between a dataset and its license(s). Where a Rights Statement refers to several licences the intention is that these should separately apply to the data and content associated with the dataset. An individual Rights Statement may be specific to a dataset or could be applied to a 
number of datasets published by the same organisation or person, where the rights associated with each dataset are identical."""@en;
    rdfs:subClassOf dct:RightsStatement.

odrs:License
    a owl:Class;    
    rdfs:isDefinedBy <http://schema.theodi.org/odrs>;
    rdfs:label "License"@en;
    rdfs:comment """A legal document that describes the legal terms for re-use of some information. A licence might be applicable to content, data, or both. It is expected that in most cases a License is a standard set of legal terms that might be used to support the publication of any number of datasets. This definition of licence used here is deliberately loose, and is intended to also cover waiver documents that indicate that the owner waives all rights over some information, e.g. public domain dedications."""@en;
    rdfs:subClassOf dct:LicenseDocument;
    owl:equivalentClass cc:License.

############################################################################
# Object Properties
############################################################################

odrs:dataLicense
    a owl:ObjectProperty;
    rdfs:isDefinedBy <http://schema.theodi.org/odrs>;
    rdfs:label "data license"@en;
    rdfs:comment "Indicates which data licence is applicable to the dataset(s) referencing a rights statement."@en;
    rdfs:subPropertyOf dct:license;
    rdfs:domain odrs:RightsStatement;
    rdfs:range odrs:License.
    
odrs:contentLicense
    a owl:ObjectProperty;
    rdfs:isDefinedBy <http://schema.theodi.org/odrs>;
    rdfs:label "content license"@en;
    rdfs:comment "Indicates which content licence is applicable to the dataset(s) referencing a rights statement"@en;
    rdfs:subPropertyOf dct:license;
    rdfs:domain odrs:RightsStatement;
    rdfs:range odrs:License.

odrs:rights
    a owl:ObjectProperty;
    rdfs:isDefinedBy <http://schema.theodi.org/odrs>;
    rdfs:label "rights"@en;
    rdfs:comment "Associates a rights statement with a dataset. This property is equivalent to the Dublin Core rights property"@en;
    owl:equivalentProperty dct:rights;
    rdfs:range odrs:RightsStatement.

odrs:reuserGuidelines
    a owl:ObjectProperty;
    rdfs:isDefinedBy <http://schema.theodi.org/odrs>;
    rdfs:label "guidelines for re-users"@en;
    rdfs:comment """Link to a document that provides guidelines for re-users of data that is covered by a specific rights statement. The guidelines 
may include more detail on attribution guidelines, a fuller copyright statement, and general guidance on how the data might be re-used"""@en;
    rdfs:domain odrs:RightsStatement;
    rdfs:range foaf:Document.

odrs:attributionURL
    a owl:ObjectProperty;
    rdfs:isDefinedBy <http://schema.theodi.org/odrs>;
    rdfs:label "attribution url"@en;
    rdfs:comment """The link which should be used when attributing a data source. The URL could be a reference to the dataset or publisher 
homepage, but may also be a dedicated attribution page. This is useful when providing onward attribution to upstream sources."""@en;    
    rdfs:domain odrs:RightsStatement;
    rdfs:range foaf:Document.

odrs:copyrightStatement
    a owl:ObjectProperty;
    rdfs:isDefinedBy <http://schema.theodi.org/odrs>;
    rdfs:label "copyright statement"@en;
    rdfs:comment """A link to a document that includes a statement about the copyright status of the content of a dataset. The web page might include both a copyright notice for a dataset, and any relevant guidance for re-users."""@en;    
    rdfs:domain odrs:RightsStatement;
    rdfs:range foaf:Document.

odrs:compatibleWith
    a owl:ObjectProperty;
    rdfs:isDefinedBy <http://schema.theodi.org/odrs>;
    rdfs:label "compatible with"@en;
    rdfs:comment """Indicates that one license is compatible with another. Here this is defined as meaning that two Licenses X and Y have the same requirements, permissions, and possibly prohibitions. 
    A user may therefore relicense data under License Y because their use will still comply with License X. Re-use that is compliant with License Y is automatically compliant with License X."""@en;    
    rdfs:domain odrs:License;
    rdfs:range odrs:License.


############################################################################
# Datatype Properties
############################################################################

odrs:copyrightHolder
    a owl:DatatypeProperty;
    rdfs:isDefinedBy <http://schema.theodi.org/odrs>;
    rdfs:label "copyright holder"@en;
    rdfs:comment """The name of the person, organisation or group that holds copyright over the dataset or its contents"""@en;    
    rdfs:range rdfs:Literal;
    rdfs:domain odrs:RightsStatement.

odrs:copyrightYear
    a owl:DatatypeProperty;
    rdfs:isDefinedBy <http://schema.theodi.org/odrs>;
    rdfs:label "copyright year"@en;
    rdfs:comment """The year from which copyright is asserted."""@en;    
    rdfs:range rdfs:Literal;
    rdfs:domain odrs:RightsStatement.

odrs:attributionText
    a owl:DatatypeProperty;
    rdfs:isDefinedBy <http://schema.theodi.org/odrs>;
    rdfs:label "attribution text"@en;
    rdfs:comment "The text to use in an attribution link. This may be the name of the publisher or a reference to a community or group of contributors"@en;    
    rdfs:range rdfs:Literal;
    rdfs:domain odrs:RightsStatement.

